wip

theories/invariant.v
@@ -5,41 +5,198 @@ Require Export diris.rtypesystem.
 Require Export diris.langlemmas.
 Require Export diris.genericinv.
 
-Fixpoint buf_typed (buf : list val) (ct : chan_type) (rest : chan_type) : rProp :=
-  match buf, ct with
-                            (* add owner here *)
-  | v::buf', RecvT t ct' => val_typed v t ∗ buf_typed buf' ct' rest
-  (* | v::buf', SendT t ct' => ??? *)
-  (* Add a rule for this to support asynchrous subtyping *)
-  | [], ct => ⌜⌜ rest = ct ⌝⌝
-  | _,_ => False
-  end.
+Section bufs_typed.
+  Fixpoint buf_typed (buf : list val) (ct : chan_type) (rest : chan_type) : rProp :=
+    match buf, ct with
+                              (* add owner here *)
+    | v::buf', RecvT t ct' => val_typed v t ∗ buf_typed buf' ct' rest
+    (* | v::buf', SendT t ct' => ??? *)
+    (* Add a rule for this to support asynchrous subtyping *)
+    | [], ct => ⌜⌜ rest = ct ⌝⌝
+    | _,_ => False
+    end.
 
-Definition bufs_typed (b1 b2 : list val) (σ1 σ2 : chan_type) : rProp :=
-  ∃ rest, buf_typed b1 σ1 rest ∗
-          buf_typed b2 σ2 (dual rest).
+  Lemma dual_dual σ : dual (dual σ) = σ.
+  Proof.
+    induction σ; simpl; rewrite ?IHσ; eauto.
+  Qed.
 
-Definition link_σ (which : bool) (b' : option (list val)) (b : list val) (σ : chan_type) : rProp :=
-  (⌜⌜ b' = Some b ⌝⌝ ∗ own_in (which,σ)) ∨ ⌜⌜ b' = None ∧ σ = EndT ∧ b = [] ⌝⌝.
+  Definition buf_typed' (buf' : option (list val)) (ct' : option chan_type) (rest : chan_type) : rProp :=
+    match buf', ct' with
+    | Some buf, Some ct => buf_typed buf ct rest
+    | None, None => emp%I
+    | _, _ => False
+    end.
 
-Definition thread_inv (e : expr) := rtyped0 e UnitT.
+  Definition bufs_typed (b1' b2' : option (list val)) (σ1' σ2' : option chan_type) : rProp :=
+    ∃ rest,
+      buf_typed' b1' σ1' rest ∗
+      buf_typed' b2' σ2' (dual rest).
+End bufs_typed.
 
-Definition chan_inv (b1' b2' : option (list val)) : rProp :=
-  ∃ σ1 σ2 b1 b2,
-    link_σ true b1' b1 σ1 ∗
-    link_σ false b2' b2 σ2 ∗
-    bufs_typed b1 b2 σ1 σ2.
+Section invariant.
+  Definition opt_to_singleton {T:ofe} (b:bool) (x : option T) : multiset (bool*T) :=
+    match x with
+    | Some a => {[ (b,a) ]}
+    | None => ε
+    end.
 
-Definition state_inv (es : list expr) (h : heap) (x : object) : rProp :=
-  match x with
-  | Thread n =>
-      rtyped0 (default (Val $ UnitV) (es !! n)) UnitT
-  | Chan n =>
-      chan_inv (h !! (n,true)) (h !! (n,false))
-  end.
+  Definition mset_σs (σs : gmap bool chan_type) : multiset clabel :=
+    opt_to_singleton true (σs !! true) ⋅ opt_to_singleton false (σs !! false).
 
-Definition invariant (es : list expr) (h : heap) :=
-  inv (state_inv es h).
+  Definition state_inv (es : list expr) (h : heap) (x : object) (in_l : multiset clabel) : rProp :=
+    match x with
+    | Thread n =>
+      ⌜⌜ in_l ≡ ε ⌝⌝ ∗
+      match es !! n with
+      | Some e => rtyped0 e UnitT
+      | None => emp
+      end
+    | Chan n => ∃ σs : gmap bool chan_type,
+      ⌜⌜ in_l ≡ mset_σs σs ⌝⌝ ∗
+      bufs_typed (h !! (n,true)) (h !! (n,false)) (σs !! true) (σs !! false)
+    end%I.
+
+  Definition invariant (es : list expr) (h : heap) := inv (state_inv es h).
+End invariant.
+
+Instance state_inv_proper es h v : Proper ((≡) ==> (⊣⊢)) (state_inv es h v).
+Proof.
+  solve_proper_prepare.
+  destruct v.
+  - solve_proper.
+  - setoid_rewrite H. done.
+Qed.
+Instance state_inv_params : Params (@state_inv) 3. Defined.
+
+Lemma bufs_typed_sym' b1' b2' σ1' σ2' :
+  bufs_typed b1' b2' σ1' σ2' ⊢
+  bufs_typed b2' b1' σ2' σ1'.
+Proof.
+  iIntros "H". unfold bufs_typed.
+  iDestruct "H" as (rest) "[H1 H2]".
+  iExists (dual rest). rewrite dual_dual. iFrame.
+Qed.
+
+Lemma bufs_typed_wlog b b' (h : heap) (σs : gmap bool chan_type) n :
+  bufs_typed (h !! (n,b)) (h !! (n,negb b)) (σs !! b) (σs !! negb b) ⊢
+  bufs_typed (h !! (n,b')) (h !! (n,negb b')) (σs !! b') (σs !! negb b').
+Proof.
+  destruct (decide (b = b')); subst; first eauto.
+  assert (negb b = b') as ->. { by destruct b,b'. }
+  assert (negb b' = b) as ->. { by destruct b,b'. }
+  by rewrite bufs_typed_sym'.
+Qed.
+
+Lemma mset_delete σs b r x :
+  {[(b, r):clabel]} ⋅ x ≡ mset_σs σs ->
+  x ≡ mset_σs (delete b σs).
+Proof.
+  intros H.
+Admitted.
+
+Lemma mset_lookup σs b r x :
+  {[(b, r):clabel]} ⋅ x ≡ mset_σs σs ->
+  σs !! b = Some r.
+Proof.
+  intros.
+  pose proof (mset_delete _ _ _ _ H).
+  assert (b = true) as -> by admit.
+  unfold mset_σs in *.
+  rewrite lookup_delete in H0.
+  rewrite lookup_delete_ne in H0; eauto.
+Admitted.
+
+Lemma mset_insert σs x b r r' :
+  {[(b, r):clabel]} ⋅ x ≡ mset_σs σs ->
+  {[(b, r'):clabel]} ⋅ x ≡ mset_σs (<[b:=r']> σs).
+Proof.
+  intros H%mset_delete. rewrite H.
+  unfold mset_σs.
+  rewrite !lookup_delete_spec.
+  rewrite !lookup_insert_spec.
+  destruct b; simpl.
+  - destruct (_ !! _); simpl; eauto.
+  - destruct (_ !! _); simpl; eauto.
+    rewrite comm. done.
+Qed.
+
+Lemma mset_empty :
+  mset_σs ∅ = ε.
+Proof.
+  unfold mset_σs. rewrite !lookup_empty. simpl. done.
+Qed.
+
+Lemma mset_empty' σs :
+  (∀ b, σs !! b = None) ->
+  mset_σs σs = ε.
+Proof.
+  intros H.
+  assert (σs = ∅) as -> by by apply map_empty.
+  apply mset_empty.
+Qed.
+
+Lemma buf_typed_push v buf t r c :
+  val_typed v t ∗
+  buf_typed buf c (RecvT t r) ⊢
+  buf_typed (buf ++ [v]) c r.
+Proof.
+  iIntros "[H1 H2]".
+  iInduction buf as [] "IH" forall (r c); simpl.
+  - iDestruct "H2" as "<-". iFrame. done.
+  - destruct c; eauto. iDestruct "H2" as "[H2 H3]".
+    iFrame. iApply ("IH" with "H1"). done.
+Qed.
+
+Lemma bufs_typed_push b1' t v buf σ2' r :
+  val_typed v t ∗
+  bufs_typed b1' (Some buf) (Some (SendT t r)) σ2' ⊢
+  bufs_typed b1' (Some (buf ++ [v])) (Some r) σ2'.
+Proof.
+  iIntros "[H1 H2]".
+  unfold bufs_typed.
+  iDestruct "H2" as (rest) "[H2 H3]".
+  destruct b1'; simpl; eauto.
+  destruct σ2'; eauto. simpl. destruct l; eauto. simpl.
+  iDestruct "H2" as "%". subst. simpl.
+  iExists r. iSplit; eauto.
+  iApply buf_typed_push. iFrame.
+Qed.
+
+Lemma bufs_typed_pop b1 b2' σ1 σ2' (v : val) t :
+  bufs_typed (Some (v :: b1)) b2' (Some (RecvT t σ1)) σ2' -∗
+  val_typed v t ∗ bufs_typed (Some b1) b2' (Some σ1) σ2'.
+Proof.
+  iIntros "H".
+  iDestruct "H" as (rest) "[H1 H2]". simpl.
+  iDestruct "H1" as "[H1 H3]". iFrame.
+  iExists rest. iFrame.
+Qed.
+
+Lemma bufs_typed_dealloc b2' σ2 :
+  bufs_typed (Some []) b2' (Some EndT) σ2 ⊢
+  bufs_typed None b2' None σ2.
+Proof.
+  iIntros "H".
+  iDestruct "H" as (rest) "[% H2]". subst.
+  iExists _. iFrame. done.
+Qed.
+
+Lemma bufs_typed_None σ1 σ2 :
+  bufs_typed None None σ1 σ2 ⊢ ⌜⌜ σ1 = None ∧ σ2 = None ⌝⌝.
+Proof.
+  iIntros "H".
+  iDestruct "H" as (rest) "[H1 H2]".
+  destruct σ1,σ2; eauto.
+Qed.
+
+Lemma bufs_typed_init r :
+  emp ⊢ bufs_typed (Some []) (Some []) (Some r) (Some (dual r)).
+Proof.
+  iIntros "H".
+  unfold bufs_typed.
+  iExists r; simpl; eauto.
+Qed.
 
 Lemma preservation (threads threads' : list expr) (chans chans' : heap) :
   step threads chans threads' chans' ->
@@ -49,42 +206,182 @@ Proof.
   intros [].
   destruct H as [????????HH].
   intros Hinv.
-  unfold invariant in *.
   destruct HH; rewrite ?right_id.
   - (* Pure step *)
     eapply inv_impl; last done.
-    iIntros (v) "H". destruct v; simpl; eauto.
+    iIntros ([] x) "H"; simpl; eauto.
+    iDestruct "H" as "[H1 H2]". iFrame.
     rewrite list_lookup_insert_spec. case_decide; eauto.
-    destruct H2; subst. rewrite H0. simpl.
-    iDestruct (typed0_ctx_typed0 with "H") as (t) "[Hctx Ht]"; eauto.
-    iApply (ctx_subst0 with "Hctx").
-    iApply pure_step_rtyped0; eauto.
+    destruct H2. subst. rewrite H0.
+    iDestruct (rtyped0_ctx with "H2") as (t) "[H1 H2]"; eauto.
+    iApply "H2". iApply pure_step_rtyped0; eauto.
   - (* Send *)
-
-    destruct c.
-    eapply (inv_exchange (v1 := Thread i) (v2 := Chan c)); last done.
-    + intros. iIntros "H". destruct v; simpl.
+    eapply (inv_exchange (Thread i) (Chan c.1)); last done; first apply _; first apply _.
+    + intros v x []. iIntros "H".
+      destruct v; simpl.
       * rewrite list_lookup_insert_spec. case_decide; naive_solver.
-      * unfold maybe_own_σ_in. rewrite !lookup_insert_spec. admit.
-    + simpl. rewrite H0. simpl.
-      iIntros "H".
-      iDestruct (typed0_ctx_typed0 with "H") as (t) "[Hctx Ht]"; eauto.
-      simpl.
-      iDestruct "Ht" as (r t' ->) "[H1 Hv]".
-      iDestruct "H1" as (r0 Heq) "H". simplify_eq.
-      iSplitL "H". iFrame. iExact "H". iFrame.
-
-      iDestruct (typed0_ct)
-    admit.
+      * setoid_rewrite lookup_insert_spec. repeat case_decide; eauto; destruct c; simpl in *; simplify_eq.
+    + iIntros (y0) "H". simpl. rewrite H0.
+      iDestruct "H" as (HH) "H".
+      iDestruct (rtyped0_ctx with "H") as (t) "[H1 H2]"; eauto. simpl.
+      iDestruct "H1" as (r t' ->) "[H1 H1']".
+      iDestruct "H1" as (r0 HH') "H1". simplify_eq.
+      destruct c. simpl.
+      iExists _. iFrame.
+      iIntros (x) "H".
+      iExists (b, r).
+      rewrite list_lookup_insert; last by eapply lookup_lt_Some.
+      iSplitL "H2".
+      * iIntros "H1".
+        iSplit; eauto.
+        iApply "H2". simpl.
+        eauto with iFrame.
+      * iDestruct "H" as (σs H2) "H".
+        iExists (<[ b := r ]> σs).
+        iSplit.
+        -- iPureIntro. by eapply mset_insert.
+        -- iApply (bufs_typed_wlog b true).
+           iDestruct (bufs_typed_wlog true b with "H") as "H".
+           assert (σs !! b = Some (SendT t' r)) as ->
+             by by eapply mset_lookup.
+           rewrite !lookup_insert_spec.
+           repeat case_decide; simplify_eq; try solve [by destruct b].
+           rewrite H1.
+           iApply bufs_typed_push. iFrame.
   - (* Receive *)
-    admit.
+    eapply (inv_exchange (Thread i) (Chan c.1)); last done; first apply _; first apply _.
+    + intros v x []. iIntros "H".
+      destruct v; simpl.
+      * rewrite list_lookup_insert_spec. case_decide; naive_solver.
+      * setoid_rewrite lookup_insert_spec. repeat case_decide; eauto; destruct c; simpl in *; simplify_eq.
+    + iIntros (y0) "H". simpl. rewrite H0.
+      iDestruct "H" as (HH) "H".
+      iDestruct (rtyped0_ctx with "H") as (t) "[H1 H2]"; eauto. simpl.
+      iDestruct "H1" as (t' r ->) "H1".
+      iDestruct "H1" as (r0 HH') "H1". simplify_eq.
+      destruct c. simpl.
+      iExists _. iFrame.
+      iIntros (x) "H".
+      iExists (b, r).
+      rewrite list_lookup_insert; last by eapply lookup_lt_Some.
+      iDestruct "H" as (σs H2) "H".
+      iDestruct (bufs_typed_wlog true b with "H") as "H".
+      assert (σs !! b = Some (RecvT t' r)) as ->
+             by by eapply mset_lookup.
+      rewrite H1.
+      iDestruct (bufs_typed_pop with "H") as "[Hv H]".
+      iSplitL "H2 Hv".
+      * iIntros "H1".
+        iSplit; eauto.
+        iApply "H2". simpl.
+        iExists _,_. iSplit; first done.
+        eauto with iFrame.
+      * iExists (<[ b := r ]> σs).
+        iSplit.
+        -- iPureIntro. by eapply mset_insert.
+        -- iApply (bufs_typed_wlog b true).
+           rewrite !lookup_insert_spec.
+           repeat case_decide; simplify_eq; try solve [by destruct b].
   - (* Close *)
-    destruct (decide (h !! other c = None)).
-    + admit.
-    + admit.
+    eapply (inv_dealloc (Thread i) (Chan c.1)); last done; first apply _; first apply _.
+    + intros v x []. iIntros "H".
+      destruct v; simpl.
+      * rewrite list_lookup_insert_spec. case_decide; naive_solver.
+      * setoid_rewrite lookup_delete_spec. repeat case_decide; eauto; destruct c; simpl in *; simplify_eq.
+    + iIntros (y0) "H". simpl. rewrite H0.
+      iDestruct "H" as (HH) "H".
+      iDestruct (rtyped0_ctx with "H") as (t) "[H1 H2]"; eauto. simpl.
+      iDestruct "H1" as (->) "H1".
+      iDestruct "H1" as (r0 HH') "H1". simplify_eq.
+      destruct c. simpl.
+      iExists _. iFrame.
+      iIntros (x) "H".
+      iDestruct "H" as (σs Hσs) "H".
+      iDestruct (bufs_typed_wlog true b with "H") as "H".
+      rewrite H1.
+      assert (σs !! b = Some EndT) as ->
+             by by eapply mset_lookup.
+      rewrite list_lookup_insert; last by eapply lookup_lt_Some.
+      (* iDestruct (bufs_typed_pop with "H") as "[Hv H]". *)
+      iSplitL "H2".
+      * iSplit; eauto. by iApply "H2".
+      * iExists (delete b σs).
+        iSplit.
+        -- iPureIntro. by eapply mset_delete.
+        -- iApply (bufs_typed_wlog b true).
+           rewrite !lookup_delete_spec.
+           repeat case_decide; simplify_eq; try solve [by destruct b].
+           by iApply bufs_typed_dealloc.
   - (* Fork *)
-    admit.
-Admitted.
+    eapply (inv_alloc_lr (Thread i) (Chan i0) (Thread (length es))); last done;
+      first apply _; first apply _.
+    + split_and!; eauto. intro. simplify_eq.
+      apply lookup_lt_Some in H0. lia.
+    + intros v' x []. iIntros "H".
+      destruct v'; simpl.
+      * rewrite lookup_app_lr.
+        rewrite list_lookup_insert_spec.
+        rewrite list_lookup_singleton_spec.
+        repeat case_decide.
+        -- naive_solver.
+        -- naive_solver.
+        -- destruct H4. exfalso. apply H7.
+           f_equal. rewrite insert_length in H6.
+           rewrite insert_length in H5. lia.
+        -- destruct H4.
+           rewrite insert_length in H6.
+           rewrite insert_length in H5.
+           assert (n > length es) by lia.
+           rewrite lookup_ge_None_2; eauto. lia.
+      * setoid_rewrite lookup_insert_spec.
+        repeat case_decide; simplify_eq.
+        destruct H4; simplify_eq.
+        rewrite !lookup_insert_ne //.
+        intro. simplify_eq.
+    + iIntros (x) "H". simpl.
+      iDestruct "H" as (σs Hσs) "H".
+      rewrite H1 H2.
+      iDestruct (bufs_typed_None with "H") as "H".
+      iDestruct "H" as "%". iPureIntro.
+      rewrite Hσs.
+      rewrite mset_empty'; first done.
+      intros []; naive_solver.
+    + iIntros (x) "[H1 H2]". simpl.
+      iFrame. destruct (es !! length es) eqn:E; eauto.
+      exfalso.
+      eapply lookup_lt_Some in E. lia.
+    + iIntros (y0) "H". simpl. rewrite H0.
+      iDestruct "H" as (HH) "H".
+      iDestruct (rtyped0_ctx with "H") as (t) "[H1 H2]"; eauto. simpl.
+      iDestruct "H1" as (r ->) "H1".
+      iExists (true,r),(false,dual r).
+      iSplitL "H2".
+      * iIntros "H". iSplit; eauto.
+        rewrite lookup_app_l. 2: {
+          rewrite insert_length.
+          eapply lookup_lt_Some; eauto.
+        }
+        rewrite list_lookup_insert; eauto using lookup_lt_Some.
+        iApply "H2". simpl.
+        eauto.
+      * iSplitL "".
+        -- iExists {[ true := r; false := dual r ]}.
+           iSplit; eauto.
+           rewrite !lookup_insert.
+           rewrite lookup_insert_ne; eauto.
+           rewrite !lookup_insert.
+           rewrite lookup_insert_ne; eauto.
+           rewrite !lookup_insert.
+           by iApply bufs_typed_init.
+        -- iIntros "H".
+           iSplit; eauto.
+           rewrite lookup_app_r. 2: {
+             by rewrite insert_length.
+           }
+           rewrite insert_length.
+           replace (length es - length es) with 0 by lia. simpl.
+           iExists _. iFrame. eauto.
+Qed.
 
 
 Lemma preservationN (threads threads' : list expr) (chans chans' : heap) :
@@ -93,4 +390,30 @@ Lemma preservationN (threads threads' : list expr) (chans chans' : heap) :
   invariant threads' chans'.
 Proof.
   induction 1; eauto using preservation.
+Qed.
+
+Lemma invariant_init (e : expr) :
+  typed ∅ e UnitT -> invariant [e] ∅.
+Proof.
+  intros H.
+  eapply inv_impl; last eauto using inv_init.
+  intros. simpl. iIntros "[% H]".
+  unfold state_inv. destruct v.
+  - destruct n; simpl.
+    + subst. iSplit; eauto.
+      iApply rtyped_rtyped0.
+      iApply typed_rtyped. done.
+    + subst. iFrame. eauto.
+  - rewrite !lookup_empty.
+    iExists ∅. unfold bufs_typed. simpl. rewrite !lookup_empty. iFrame.
+    iSplit.
+    + iPureIntro. subst. unfold mset_σs.
+      rewrite !lookup_empty. simpl. done.
+    + iExists EndT. done.
+Qed.
+
+Lemma invariant_holds e threads chans :
+  typed ∅ e UnitT -> steps [e] ∅ threads chans -> invariant threads chans.
+Proof.
+  eauto using invariant_init, preservationN.
 Qed.
