theories/legacy/invariant.v
@@ -1,0 +1,96 @@
+Require Export diris.langdef.
+Require Export diris.cgraph.
+Require Export diris.seplogic.
+Require Export diris.rtypesystem.
+Require Export diris.langlemmas.
+Require Export diris.genericinv.
+
+Fixpoint buf_typed (buf : list val) (ct : chan_type) (rest : chan_type) : rProp :=
+  match buf, ct with
+                            (* add owner here *)
+  | v::buf', RecvT t ct' => val_typed v t ∗ buf_typed buf' ct' rest
+  (* | v::buf', SendT t ct' => ??? *)
+  (* Add a rule for this to support asynchrous subtyping *)
+  | [], ct => ⌜⌜ rest = ct ⌝⌝
+  | _,_ => False
+  end.
+
+Definition bufs_typed (b1 b2 : list val) (σ1 σ2 : chan_type) : rProp :=
+  ∃ rest, buf_typed b1 σ1 rest ∗
+          buf_typed b2 σ2 (dual rest).
+
+Definition link_σ (which : bool) (b' : option (list val)) (b : list val) (σ : chan_type) : rProp :=
+  (⌜⌜ b' = Some b ⌝⌝ ∗ own_in (which,σ)) ∨ ⌜⌜ b' = None ∧ σ = EndT ∧ b = [] ⌝⌝.
+
+Definition thread_inv (e : expr) := rtyped0 e UnitT.
+
+Definition chan_inv (b1' b2' : option (list val)) : rProp :=
+  ∃ σ1 σ2 b1 b2,
+    link_σ true b1' b1 σ1 ∗
+    link_σ false b2' b2 σ2 ∗
+    bufs_typed b1 b2 σ1 σ2.
+
+Definition state_inv (es : list expr) (h : heap) (x : object) : rProp :=
+  match x with
+  | Thread n =>
+      rtyped0 (default (Val $ UnitV) (es !! n)) UnitT
+  | Chan n =>
+      chan_inv (h !! (n,true)) (h !! (n,false))
+  end.
+
+Definition invariant (es : list expr) (h : heap) :=
+  inv (state_inv es h).
+
+Lemma preservation (threads threads' : list expr) (chans chans' : heap) :
+  step threads chans threads' chans' ->
+  invariant threads chans ->
+  invariant threads' chans'.
+Proof.
+  intros [].
+  destruct H as [????????HH].
+  intros Hinv.
+  unfold invariant in *.
+  destruct HH; rewrite ?right_id.
+  - (* Pure step *)
+    eapply inv_impl; last done.
+    iIntros (v) "H". destruct v; simpl; eauto.
+    rewrite list_lookup_insert_spec. case_decide; eauto.
+    destruct H2; subst. rewrite H0. simpl.
+    iDestruct (typed0_ctx_typed0 with "H") as (t) "[Hctx Ht]"; eauto.
+    iApply (ctx_subst0 with "Hctx").
+    iApply pure_step_rtyped0; eauto.
+  - (* Send *)
+
+    destruct c.
+    eapply (inv_exchange (v1 := Thread i) (v2 := Chan c)); last done.
+    + intros. iIntros "H". destruct v; simpl.
+      * rewrite list_lookup_insert_spec. case_decide; naive_solver.
+      * unfold maybe_own_σ_in. rewrite !lookup_insert_spec. admit.
+    + simpl. rewrite H0. simpl.
+      iIntros "H".
+      iDestruct (typed0_ctx_typed0 with "H") as (t) "[Hctx Ht]"; eauto.
+      simpl.
+      iDestruct "Ht" as (r t' ->) "[H1 Hv]".
+      iDestruct "H1" as (r0 Heq) "H". simplify_eq.
+      iSplitL "H". iFrame. iExact "H". iFrame.
+
+      iDestruct (typed0_ct)
+    admit.
+  - (* Receive *)
+    admit.
+  - (* Close *)
+    destruct (decide (h !! other c = None)).
+    + admit.
+    + admit.
+  - (* Fork *)
+    admit.
+Admitted.
+
+
+Lemma preservationN (threads threads' : list expr) (chans chans' : heap) :
+  steps threads chans threads' chans' ->
+  invariant threads chans ->
+  invariant threads' chans'.
+Proof.
+  induction 1; eauto using preservation.
+Qed.
