theories/progress.v
@@ -1,0 +1,83 @@
+From diris Require Import invariant.
+(*
+  Local progress: if e is well typed, then in all heaps that are well typed
+   (and consistent with the heap typing for e), then either:
+   - e can take a step in that heap
+   - e is a value
+   - e is waiting to receive on a channel with an empty buffer
+*)
+
+Lemma local_progress : True. Admitted.
+
+(*
+  Global progress: if the invariant holds for (es,h) then either:
+  - all e ∈ es are unit, and h = ∅
+  - the configuration can step
+*)
+
+Lemma is_unit_decision e :
+  Decision (e = Val UnitV).
+Proof.
+  destruct e; try solve [right; intro; simplify_eq].
+  destruct v; try solve [right; intro; simplify_eq].
+  left. done.
+Qed.
+
+Lemma exprs_decision (es : list expr) :
+  Decision (∃ e, e ∈ es ∧ e ≠ Val UnitV).
+Proof.
+  eapply (dec_exists_list _ es).
+  - intros ? []; eauto.
+  - intros.
+    destruct (is_unit_decision x); subst.
+    + right. intros []. apply H1. done.
+    + left. eauto.
+Qed.
+
+Lemma heap_decision (h : heap) :
+  Decision (∃ c, is_Some (h !! c)).
+Proof.
+  destruct (decide (h = ∅)).
+  - right. intros []. subst. rewrite lookup_empty in H.
+    destruct H. simplify_eq.
+  - left. destruct (map_to_list h) eqn:E.
+    { apply map_to_list_empty_inv in E. subst. exfalso.
+      apply n. done. }
+    destruct p.
+    exists e.
+    assert ((e,l0) ∈ map_to_list h).
+    { rewrite E. rewrite elem_of_cons. eauto. }
+    apply elem_of_map_to_list in H. rewrite H. eauto.
+Qed.
+
+Lemma final_state_decision (es : list expr) (h : heap) :
+  {(∃ c, is_Some (h !! c)) ∨ (∃ e, e ∈ es ∧ e ≠ Val UnitV)} +
+  {h = ∅ ∧ ∀ e, e ∈ es -> e = Val UnitV}.
+Proof.
+  destruct (heap_decision h); [left; eauto|].
+  destruct (exprs_decision es); [left; eauto|].
+  right. split.
+  - assert (∀ c, ¬ is_Some (h !! c)) by naive_solver.
+    assert (∀ c, h !! c = None).
+    { intros. destruct (h !! c) eqn:E; eauto.
+      exfalso. eapply H. erewrite E. eauto. }
+    apply map_empty. eauto.
+  - intros.
+    assert (∀ e, ¬ (e ∈ es ∧ e ≠ Val UnitV)) by naive_solver.
+    specialize (H0 e).
+    destruct (is_unit_decision e); eauto.
+    exfalso.
+    apply H0; eauto.
+Qed.
+
+Lemma global_progress es h :
+  invariant es h ->
+  (h = ∅ ∧ ∀ e, e ∈ es -> e = Val UnitV) ∨
+  (∃ es' h', step es h es' h').
+Proof.
+  intros H.
+  destruct (final_state_decision es h) as [Hdec|Hdec]; eauto.
+  right.
+
+
+Admitted.
