theories/todo.md
@@ -26,3 +26,7 @@
   - async subtyping
   - locks
 * write paper
+
+ ∀ h, P(h) -> Q(<[x:=v]> h)
+-----------------------
+   {P} x := v {Q}
